

# How to not to be a coward

I saw the following proof today (from [Twitter](https://x.com/VinceVatter/status/1882125739111448580) (https://x.com/VinceVatter/status/1882125739111448580), and also from my friend):

**Theorem.** *If  $n$  is an integer and  $n^2$  is even, then  $n$  is itself even.*

**Proof.** Contrapositives are for cowards, so assume that  $n$  is an integer and  $n^2$  is even. Then  $n^2 = 2k$  for some integer  $k$ , and thus  $n^2 - 2k = 0$ . Behold:

$$n = n + (n^2 - 2k) = n(n + 1) - 2k.$$

Both  $n(n + 1)$  and  $2k$  are even, so  $n$  is even too. **QED.**

Contrapositives are for cowards.

Now, here's a question: consider a multiple of 3 instead. We still have  $n^2 \equiv 0 \pmod{3} \Rightarrow n \equiv 0 \pmod{3}$ . Can we prove this, but not being a coward? How about mod 5?

The answer is yes. Try to do it yourself before you click the triangle below.

► Proof

In this post, we will show that similar proof works for all prime and higher powers:

**Theorem.** *For prime  $p$ ,  $\mathbb{Z}/p\mathbb{Z}$  has no nilpotent elements. In other words, for  $k \geq 2$ ,  $n^k \equiv 0 \pmod{p}$  implies  $n \equiv 0 \pmod{p}$ .*

First of all, we can reduce to the case when  $k = 2$ . For given  $k$ , take  $a$  with  $2^a \geq k$ . Then we have  $n^{2^a} = (n^{2^{a-k}})^{2^k} \equiv 0 \pmod{p}$ . From  $n^{2^a} = (n^{2^{a-1}})^2$ , we have  $n^{2^{a-1}} \equiv 0 \pmod{p}$ , and repeating this gives  $n \equiv 0 \pmod{p}$ .

For  $k = 2$ , our goal is to express  $n$  as a  $\mathbb{Z}$ -linear combination of integer-valued polynomials, which are (i) divisible by  $n^2$ , or (ii) every value is divisible by  $p$ . As above,

$$\begin{aligned} f(n) &= n(n+1)(n+2) \cdots (n+(p-1)) \\ &= n^p + a_{p-1} n^{p-1} + \cdots + a_2 n^2 + a_1 n \end{aligned}$$

is a multiple of  $p$  for any  $n$ . We have  $a_1 = (p-1)!$ , and by Wilson's theorem

([https://en.wikipedia.org/wiki/Wilson%27s\\_theorem](https://en.wikipedia.org/wiki/Wilson%27s_theorem)),  $a_1 + 1 = (p-1)! + 1$  is a multiple of  $p$ . Hence

$$n = n^2(n^{p-2} + a_{p-1}n^{p-3} + \cdots + a_2) + (a_1 + 1)n - f(n)$$

is divisible by  $p$ .  $\square$


The theorem is still true if one replace  $p$  with square-free integers. In fact, the decomposition for  $p = 3$  gives a proof for mod 6, too. Unfortunately, I don't know if there's a general construction of a combination for square-free modulus case.

0 Comments - powered by *utteranc.es*

Write

Preview

Sign in to comment

 Styling with Markdown is supported
 

Sign in with GitHub

Tags: math